\chapter{Derivation of CEC}
\label{appc}

Certainty equivalent consumption is a level of consumption which corresponds to deterministic utility which is exactly equal to the expected utility. We have:

\begin{center}
	$U(CEC) = E[U(c)]$
\end{center}

Substituting the formulas gives:

\begin{center}
	$\displaystyle\sum^T_{t=1} \delta^{t-1} \displaystyle\prod^{t-1}_{j=0} p_j \cdot \frac{CEC^{1-\gamma}}{1-\gamma}\right] = E[U(c)]$
\end{center}

Leaving $CEC$ alone gives the desired outcome:

\begin{center}
	$CEC = \left( \frac{E[U(c)]\cdot(1-\gamma)}{\sum^T_{t=1} \delta^{t-1} \prod^{t-1}_{j=0} p_j} \right)^{1/(1-\gamma)}$
\end{center}


